steel/Zeta.Steel.GhostSharedMap.fsti
@@ -1,0 +1,527 @@
+module Zeta.Steel.GhostSharedMap
+open Steel.ST.Util
+open FStar.Map
+open FStar.PCM
+open FStar.Preorder
+open Steel.Preorder
+open Zeta.Steel.Util
+open FStar.TSet
+open Steel.FractionalPermission
+#push-options "--z3cliopt 'smt.qi.eager_threshold=100' --fuel 0 --ifuel 2 --z3rlimit_factor 4"
+let kmap (k:eqtype) (v:Type) (p:preorder v) =
+  Map.t k (option perm & vhist p)
+
+#push-options "--fuel 1"
+let initial_map (#k:eqtype) (#v:Type) (#p:preorder v)
+                (f:option perm) (value:v)
+  : kmap k v p
+  = map_literal (fun _ -> f, ([value] <: vhist p))
+#pop-options
+
+[@@erasable]
+noeq
+type knowledge (k:eqtype) (v:Type) (p:preorder v) =
+  | Full     : kmap k v p -> knowledge k v p
+  | Owns     : kmap k v p -> knowledge k v p
+  | Nothing  : knowledge k v p
+
+let b2p (b:bool)
+  : prop
+  = b == true
+
+let perm_opt_composable (p0 p1:option perm)
+  : prop
+  = match p0, p1 with
+    | None, None -> True
+    | Some p, None
+    | None, Some p -> b2p (p `lesser_equal_perm` full)
+    | Some p0, Some p1 -> b2p (sum_perm p0 p1 `lesser_equal_perm` full)
+
+let kmap_composable_k (#k:eqtype) (#v:Type) (#p:preorder v) (m0 m1: kmap k v p)
+                      (key:k)
+   : prop
+   = match Map.sel m0 key, Map.sel m1 key with
+     | (None, v0), (None, v1) ->
+       p_composable _ v0 v1
+
+     | (Some p, v), (None, v')
+     | (None, v'), (Some p, v) ->
+       v `extends` v' /\
+       perm_opt_composable (Some p) None
+
+     | (Some p0, v0), (Some p1, v1) ->
+        perm_opt_composable (Some p0) (Some p1) /\
+        v0 == v1
+
+let kmap_composable (#k:eqtype) (#v:Type) (#p:preorder v) (m0 m1: kmap k v p)
+   : prop
+   = forall k. kmap_composable_k m0 m1 k
+
+let full_kmap_composable_k (#k:eqtype) (#v:Type) (#p:preorder v) (full:kmap k v p) (m1: kmap k v p) (key:k)
+  : prop
+  = let p0, v0 = Map.sel full key in
+    let p1, v1 = Map.sel m1 key in
+    perm_opt_composable p0 p1   /\
+    (match p1 with
+     | None -> v0 `extends` v1
+     | Some _ -> v0 == v1)
+
+let full_kmap_composable (#k:eqtype) (#v:Type) (#p:preorder v) (full:kmap k v p) (m1: kmap k v p)
+  : prop
+  = forall k. full_kmap_composable_k full m1 k
+
+let composable #k #v #p
+  : symrel (knowledge k v p)
+  = fun (k0 k1:knowledge k v p) ->
+    match k0, k1 with
+    | Nothing, _
+    | _, Nothing -> True
+
+    | Full _, Full _ ->
+      False
+
+    | Full m, Owns m'
+    | Owns m', Full m ->
+      full_kmap_composable m m'
+
+    | Owns m, Owns m' ->
+      kmap_composable m m'
+
+let p_op (#a: Type u#a) (q:preorder a) (x:vhist q) (y:vhist q{p_composable q x y}) : vhist q =
+  p_op _ x y
+
+let compose_kmaps (#k:eqtype) (#v:Type) (#p:preorder v)
+                 (m0: kmap k v p)
+                 (m1: kmap k v p { kmap_composable m0 m1 })
+  : kmap k v p
+  =  map_literal
+          (fun k ->
+            match Map.sel m0 k, Map.sel m1 k with
+            | (None, v0), (None, v1) ->
+               None, p_op _ v0 v1
+
+            | (Some p, v), (None, _)
+            | (None, _), (Some p, v) ->
+              Some p, v
+
+            | (Some p0, v0), (Some p1, _) ->
+              Some (sum_perm p0 p1), v0)
+
+
+let compose_kmaps_comm (#k:eqtype) (#v:Type) (#p:preorder v)
+                       (m0: kmap k v p)
+                       (m1: kmap k v p { kmap_composable m0 m1 })
+ : Lemma (compose_kmaps m0 m1 `Map.equal` compose_kmaps m1 m0)
+         [SMTPat (compose_kmaps m0 m1);
+          SMTPat (compose_kmaps m1 m0)]
+ = ()
+
+let compose_maps_assoc (#k:eqtype) (#v:Type) (#p:preorder v)
+                       (m0: kmap k v p)
+                       (m1: kmap k v p)
+                       (m2: kmap k v p {
+                         kmap_composable m1 m2 /\
+                         kmap_composable m0 (compose_kmaps m1 m2)
+                       })
+ : Lemma (kmap_composable m0 m1 /\
+          kmap_composable (compose_kmaps m0 m1) m2 /\
+          compose_kmaps m0 (compose_kmaps m1 m2) `Map.equal`
+          compose_kmaps (compose_kmaps m0 m1) m2)
+         [SMTPat (compose_kmaps (compose_kmaps m0 m1) m2);
+          SMTPat (compose_kmaps m0 (compose_kmaps m2 m2))]
+ = ()
+
+
+let compose_maps_assoc_r (#k:eqtype) (#v:Type) (#p:preorder v)
+                       (m0: kmap k v p)
+                       (m1: kmap k v p)
+                       (m2: kmap k v p {
+                         kmap_composable m0 m1 /\
+                         kmap_composable (compose_kmaps m0 m1) m2
+                       })
+ : Lemma (kmap_composable m1 m2 /\
+          kmap_composable m0 (compose_kmaps m1 m2) /\
+          compose_kmaps m0 (compose_kmaps m1 m2) `Map.equal`
+          compose_kmaps (compose_kmaps m0 m1) m2)
+         [SMTPat (compose_kmaps (compose_kmaps m0 m1) m2);
+          SMTPat (compose_kmaps m0 (compose_kmaps m2 m2))]
+ = ()
+
+let compose #k #v #p (k0:knowledge k v p)
+                     (k1:knowledge k v p { composable k0 k1 })
+  : knowledge k v p
+  = match k0, k1 with
+    | Nothing, k
+    | k, Nothing -> k
+
+    | Full m, Owns m'
+    | Owns m', Full m ->
+      Full (compose_kmaps m m')
+
+    | Owns m, Owns m' ->
+      Owns (compose_kmaps m m')
+
+let kmap_composable_assoc_l #k #v #p (k0 k1 k2: kmap k v p)
+  : Lemma
+    (requires
+           kmap_composable k1 k2 /\
+           kmap_composable k0 (compose_kmaps k1 k2))
+    (ensures
+           kmap_composable k0 k1 /\
+           kmap_composable (compose_kmaps k0 k1) k2)
+  = ()
+
+let kmap_composable_assoc_r #k #v #p (k0 k1 k2: kmap k v p)
+  : Lemma
+    (requires
+           kmap_composable k0 k1 /\
+           kmap_composable (compose_kmaps k0 k1) k2)
+    (ensures
+           kmap_composable k1 k2 /\
+           kmap_composable k0 (compose_kmaps k1 k2))
+  = ()
+
+
+let full_kmap_composable_assoc_r_0 #k #v #p (k0 k1 k2: kmap k v p)
+  : Lemma
+    (requires
+           full_kmap_composable k0 k1 /\
+           full_kmap_composable (compose_kmaps k0 k1) k2)
+    (ensures
+           kmap_composable k1 k2 /\
+           full_kmap_composable k0 (compose_kmaps k1 k2))
+  = ()
+
+
+let full_kmap_composable_assoc_r_1 #k #v #p (k0 k1 k2: kmap k v p)
+  : Lemma
+    (requires
+           full_kmap_composable k1 k0 /\
+           full_kmap_composable (compose_kmaps k0 k1) k2)
+    (ensures
+           full_kmap_composable k1 k2 /\
+           full_kmap_composable (compose_kmaps k1 k2) k0)
+  = ()
+
+let full_kmap_composable_assoc_r_2 #k #v #p (k0 k1 k2: kmap k v p)
+  : Lemma
+    (requires
+           kmap_composable k1 k0 /\
+           full_kmap_composable k2 (compose_kmaps k0 k1))
+    (ensures
+           full_kmap_composable k2 k1 /\
+           full_kmap_composable (compose_kmaps k1 k2) k0)
+  = ()
+
+
+
+let full_kmap_composable_assoc_l_0 #k #v #p (k0 k1 k2: kmap k v p)
+  : Lemma
+    (requires
+           kmap_composable k1 k2 /\
+           full_kmap_composable k0 (compose_kmaps k1 k2))
+    (ensures
+           full_kmap_composable k0 k1 /\
+           full_kmap_composable (compose_kmaps k0 k1) k2)
+  = ()
+
+
+let full_kmap_composable_assoc_l_1 #k #v #p (k0 k1 k2: kmap k v p)
+  : Lemma
+    (requires
+           full_kmap_composable k1 k2 /\
+           full_kmap_composable (compose_kmaps k1 k2) k0)
+    (ensures
+           full_kmap_composable k1 k0 /\
+           full_kmap_composable (compose_kmaps k0 k1) k2)
+  = ()
+
+let full_kmap_composable_assoc_l_2 #k #v #p (k0 k1 k2: kmap k v p)
+  : Lemma
+    (requires
+           full_kmap_composable k2 k1 /\
+           full_kmap_composable (compose_kmaps k1 k2) k0)
+    (ensures
+           kmap_composable k1 k0 /\
+           full_kmap_composable k2 (compose_kmaps k0 k1))
+  = ()
+
+let composable_assoc_r #k #v #p (k0 k1 k2: knowledge k v p)
+  : Lemma
+    (requires  composable k0 k1 /\
+               composable (compose k0 k1) k2)
+    (ensures
+               composable k1 k2 /\
+               composable k0 (compose k1 k2))
+  = match k0, k1, k2 with
+    | Nothing, _, _
+    | _, Nothing, _
+    | _, _, Nothing -> ()
+    | _ ->
+      (match k0 with
+       | Full m0 -> (
+         match k1, k2 with
+         | Owns m1, Owns m2 ->
+           full_kmap_composable_assoc_r_0 m0 m1 m2
+         | Owns m1, Full m2 -> ()
+         | Full m1, Owns m2 -> ()
+         | Full m1, Full m2 -> ()
+       )
+
+       | Owns m0 -> (
+         match k1, k2 with
+         | Owns m1, Owns m2 ->
+           kmap_composable_assoc_r m0 m1 m2
+         | Owns m1, Full m2 ->
+           full_kmap_composable_assoc_r_2 m0 m1 m2
+         | Full m1, Owns m2 ->
+           full_kmap_composable_assoc_r_1 m0 m1 m2
+         | Full m1, Full m2 -> ()
+       )
+      )
+
+
+let composable_assoc_l #k #v #p (k0 k1 k2: knowledge k v p)
+  : Lemma
+    (requires
+               composable k1 k2 /\
+               composable k0 (compose k1 k2))
+    (ensures   composable k0 k1 /\
+               composable (compose k0 k1) k2)
+  = match k0, k1, k2 with
+    | Nothing, _, _
+    | _, Nothing, _
+    | _, _, Nothing -> ()
+    | _ ->
+      (match k0 with
+       | Full m0 -> (
+         match k1, k2 with
+         | Owns m1, Owns m2 ->
+           full_kmap_composable_assoc_l_0 m0 m1 m2
+         | Owns m1, Full m2 -> ()
+         | Full m1, Owns m2 -> ()
+         | Full m1, Full m2 -> ()
+       )
+
+       | Owns m0 -> (
+         match k1, k2 with
+         | Owns m1, Owns m2 ->
+           kmap_composable_assoc_l m0 m1 m2
+         | Owns m1, Full m2 ->
+           full_kmap_composable_assoc_l_2 m0 m1 m2
+         | Full m1, Owns m2 ->
+           full_kmap_composable_assoc_l_1 m0 m1 m2
+         | Full m1, Full m2 -> ()
+       )
+      )
+
+
+let p0 #k #v #p : pcm' (knowledge k v p) = {
+  composable;
+  op=compose;
+  one=Nothing
+}
+
+let kmap_of_knowledge #k #v #p (kn:knowledge k v p { ~(Nothing? kn) })
+  : GTot (kmap k v p)
+  = match kn with
+    | Owns m
+    | Full m -> m
+
+
+let pcm #k #v #p : pcm (knowledge k v p) = {
+  p = p0;
+  comm = (fun _ _ -> ());
+  assoc = (fun k0 k1 k2 ->
+             composable_assoc_l k0 k1 k2;
+             match k0, k1, k2 with
+             | Nothing, _, _
+             | _, Nothing, _
+             | _, _, Nothing -> ()
+             | _ ->
+               compose_maps_assoc (kmap_of_knowledge k0)
+                                  (kmap_of_knowledge k1)
+                                  (kmap_of_knowledge k2));
+  assoc_r = (fun k0 k1 k2 ->
+               composable_assoc_r k0 k1 k2;
+               match k0, k1, k2 with
+               | Nothing, _, _
+               | _, Nothing, _
+               | _, _, Nothing -> ()
+               | _ ->
+                 compose_maps_assoc_r (kmap_of_knowledge k0)
+                                      (kmap_of_knowledge k1)
+                                      (kmap_of_knowledge k2));
+  is_unit = (fun _ -> ());
+  refine = (fun x -> Full? x == true);
+}
+
+let tmap (k:eqtype) (v:Type0) (c:preorder v) = Map.t k (hist c)
+
+
+let kmap_perm_of (#k:eqtype)
+                 (#v:Type)
+                 (#p:preorder v)
+                 (m:kmap k v p)
+                 (key:k)
+    = fst (Map.sel m key)
+
+let kmap_owns_key (#k:eqtype)
+                  (#v:Type)
+                  (#p:preorder v)
+                  (m:kmap k v p)
+                  (key:k)
+    = kmap_perm_of m key == Some full
+
+let kmap_value_of (#k:eqtype)
+                  (#v:Type)
+                  (#p:preorder v)
+                  (m:kmap k v p)
+                  (key:k)
+    = snd (Map.sel m key)
+
+let kmap_update_key (#k:eqtype)
+                    (#v:Type)
+                    (#p:preorder v)
+                    (m:kmap k v p)
+                    (key:k)
+                    (value:vhist p)
+    = Map.upd m key (kmap_perm_of m key, value)
+
+let update_key (#k:eqtype)
+               (#v:Type)
+               (#p:preorder v)
+               (m:kmap k v p)
+               (key:k)
+               (v1:vhist p {
+                 kmap_owns_key m key /\
+                 v1 `extends` kmap_value_of m key
+               })
+  : frame_preserving_upd pcm (Owns m) (Owns (kmap_update_key m key v1))
+  = fun full_v ->
+      assert (Full? full_v);
+      assert (compatible pcm (Owns m) full_v);
+      let Full full_m = full_v in
+      let res = Full (kmap_update_key full_m key v1) in
+      let m' = (kmap_update_key m key v1) in
+      eliminate exists frame. composable (Owns m) frame /\ compose frame (Owns m) == full_v
+      returns (compatible pcm (Owns (kmap_update_key m key v1)) res)
+      with _. (
+           assume (composable (Owns (kmap_update_key m key v1)) frame);
+           assume (compose frame (Owns (kmap_update_key m key v1)) == res)
+      );
+      assert (compatible pcm (Owns (kmap_update_key m key v1)) res);
+      assume (forall (frame:_{composable (Owns m) frame}).
+                composable (Owns m') frame /\
+                (compose (Owns m) frame == full_v ==> compose (Owns m') frame == res));
+      res
+
+
+val t (k:eqtype) (v:Type0) (c:preorder v) : Type0
+
+val k_of (#k:eqtype) (#v:Type0) (#c:preorder v)
+         (t:t k v c)
+         (knowledge: knowledge k v c)
+  : vprop
+
+val share  (#o:_)
+           (#k:eqtype) (#v:Type0) (#c:preorder v)
+           (#m0 :kmap k v c)
+           (#m1: kmap k v c { kmap_composable m0 m1 })
+           (t:t k v c)
+  : STGhostT unit o
+    (k_of t (Owns (compose_kmaps m0 m1)))
+    (fun _ -> k_of t (Owns m0) `star` k_of t (Owns m1))
+
+val gather (#o:_)
+           (#k:eqtype) (#v:Type0) (#c:preorder v)
+           (#m0 #m1: kmap k v c)
+           (t:t k v c)
+  : STGhostT (_:unit { kmap_composable m0 m1 }) o
+    (k_of t (Owns m0) `star` k_of t (Owns m1))
+    (fun _ -> k_of t (Owns (compose_kmaps m0 m1)))
+
+let ksnapshot (#k:eqtype) (#v:Type0) (#c:preorder v)
+             (m: kmap k v c)
+  : kmap k v c
+  = map_literal (fun k -> None, snd (Map.sel m k))
+
+let snapshot (#k:eqtype) (#v:Type0) (#c:preorder v)
+             (m: kmap k v c)
+  : Map.t k v
+  = map_literal (fun k -> curval (snd (Map.sel m k)))
+
+let global_snapshot (#k:eqtype) (#v:Type0) (#c:preorder v)
+                    (t:t k v c)
+                    (m: Map.t k v)
+  : vprop
+  = exists_ (fun (km:kmap k v c) ->
+        pure (snapshot km == m) `star`
+        k_of t (Owns (ksnapshot km)))
+
+val take_snapshot (#o:_)
+                  (#k:eqtype) (#v:Type0) (#c:preorder v)
+                  (#m: kmap k v c)
+                  (t:t k v c)
+  : STGhostT unit o
+    (k_of t (Owns m))
+    (fun _ -> k_of t (Owns m) `star` global_snapshot t (snapshot m))
+
+let owns_key (#k:eqtype) (#v:Type0) (#c:preorder v)
+             (t:t k v c)
+             (key:k)
+             (perm:perm)
+             (value:v)
+  = exists_ (fun (m:kmap k v c) ->
+       pure ((forall key'. (key<>key' ==> fst (Map.sel m key') == None)) /\
+             (match Map.sel m key with
+              | None, _ -> False
+              | Some p, h ->
+                perm == p /\
+                curval h == value)) `star`
+       k_of t (Owns m))
+
+let snapshot_of_key (#k:eqtype) (#v:Type0) (#c:preorder v)
+                    (t:t k v c)
+                    (key:k)
+                    (value:v)
+  = exists_ (fun (m:kmap k v c) ->
+       pure ((forall key'. fst (Map.sel m key') == None) /\
+             (match Map.sel m key with
+              | Some _, _ -> False
+              | None, h -> curval h == value)) `star`
+       k_of t (Owns m))
+
+val local_snapshot (#o:_)
+                   (#k:eqtype) (#v:Type0) (#c:preorder v)
+                   (#key:k) (#frac:_) (#value:v)
+                   (t:t k v c)
+  : STGhostT unit o
+    (owns_key t key frac value)
+    (fun _ -> owns_key t key frac value `star` snapshot_of_key t key value)
+
+val dup_snapshot (#o:_)
+                 (#k:eqtype) (#v:Type0) (#c:preorder v)
+                 (#key:k) (#value:v)
+                 (t:t k v c)
+  : STGhostT unit o
+    (snapshot_of_key t key value)
+    (fun _ -> snapshot_of_key t key value `star` snapshot_of_key t key value)
+
+val update (#o:_)
+           (#k:eqtype) (#v:Type0) (#c:preorder v)
+           (#key:k) (#value:v)
+           (t:t k v c)
+           (value':v {c value value'})
+  : STGhostT unit o
+    (owns_key t key full_perm value)
+    (fun _ -> owns_key t key full_perm value')
+
+val update_global_snapshot (#o:_)
+                           (#k:eqtype) (#v:Type0) (#c:preorder v)
+                           (#key:k) (#frac:_) (#value:v)
+                           (t:t k v c)
+                           (m:Map.t k v)
+  : STGhostT unit o
+    (owns_key t key frac value `star` global_snapshot t m)
+    (fun _ -> owns_key t key frac value `star` global_snapshot t (Map.upd m key value))
